WIP

src/example/ClientSpinlock2.v
@@ -42,6 +42,7 @@ Module ClientSpinlock2.
                                 else Ret (inl tt));;
                            Ret r) tt);;
         _ <- (trigger Yield;;; Spinlock.unlock X);;
+        _ <- trigger Yield;;
         Ret (SCMem.val_nat 0).
 
     Definition omod : Mod.t :=
@@ -466,7 +467,170 @@ Section SIM.
     }
   Qed.
 
-  Lemma loop_case3 
+  Lemma data_case3_after n tid2 ℓL ℓl γX γe κs κl γκl γr γκw γκu :
+    ⊢
+      (▿ γκl γκw)
+      -∗
+      (▿ γκw γκu)
+      -∗
+      (▿ γr 0)
+      -∗
+      (△ γκu (1 / 2))
+      -∗
+      (prop n (clientSpinlock2_inv n tid2 ℓL ℓl γX γe κs κl γκl γr))
+      -∗
+      ((○ γX 1) ∗ (D ↦ 1) ∗ (△ γκu (1/2)) ∗ (△ γκu (1/2))).
+  Proof.
+    iIntros "#Dl #Dw #Dr Lu CL".
+    iEval (unfold clientSpinlock2_inv; simpl; red_tl_all; simpl) in "CL".
+    iDestruct "CL" as "[CL1 | [CL2 | [CL3 | CL4]]]".
+    - iDestruct "CL1" as "(_ & _ & _ & Ll & _)".
+      iPoseProof (OneShots.pending_not_shot with "Ll Dl") as "%F". inv F.
+    - iDestruct "CL2" as "(_ & _ & % & CL2)".
+      iEval (red_tl) in "CL2". iDestruct "CL2" as "(% & CL2)".
+      iEval (red_tl_all; simpl) in "CL2". iDestruct "CL2" as "(_ & Lw & #Dl2 & _)".
+      iPoseProof (OneShots.shot_agree with "Dl Dl2") as "%EQ". subst x0.
+      iPoseProof (OneShots.pending_not_shot with "Lw Dw") as "%F". inv F.
+    - iDestruct "CL3" as "(LXw & PTD & % & CL2)".
+      iEval (red_tl) in "CL2". iDestruct "CL2" as "(% & CL2)".
+      iEval (red_tl) in "CL2". iDestruct "CL2" as "(% & CL2)".
+      iEval (red_tl_all; simpl) in "CL2". iDestruct "CL2" as "(_ & Lu2 & _ & Dl2 & Dw2 & _)".
+      iPoseProof (OneShots.shot_agree with "Dl Dl2") as "%EQ". subst x.
+      iPoseProof (OneShots.shot_agree with "Dw Dw2") as "%EQ". subst x1.
+      iFrame.
+    - iDestruct "CL4" as "(_ & _ & % & CL4)".
+      iEval (red_tl) in "CL4". iDestruct "CL4" as "(% & CL4)".
+      iEval (red_tl_all; simpl) in "CL4". iDestruct "CL4" as "(Dl2 & Dw2 & Dr2 & Du)".
+      iPoseProof (OneShots.shot_agree with "Dl Dl2") as "%EQ". subst x.
+      iPoseProof (OneShots.shot_agree with "Dw Dw2") as "%EQ". subst x0.
+      iPoseProof (OneShots.pending_not_shot with "Lu Du") as "%F". inv F.
+  Qed.
+
+  Lemma loop_case3_in
+        (tid2 n ℓL ℓl : nat)
+        (LAYER_L : ℓL = 3)
+        (LAYER_l : ℓl = 2)
+        (γX γe κs κl γκl γr : nat)
+        (γκw κu γκu : nat)
+    :
+    ⊢
+      (inv n N_ClientSpinlock2 (clientSpinlock2_inv n tid2 ℓL ℓl γX γe κs κl γκl γr))
+      -∗
+      (⟦(syn_tgt_interp_as n sndl (λ m : SCMem.t, s_memory_black m))%S, 1+n⟧)
+      -∗
+      (⟦ isSpinlock n X γX γe κs ℓL, n ⟧)
+      -∗
+      (⟦((TID(tid2))
+           ∗
+           (-[κu](0)-◇ (▿ γκu 0)%S)
+           ∗
+           (κu -(0)-◇ κs)
+           ∗
+           (▿ γκl γκw)
+           ∗
+           (▿ γκw γκu)
+           ∗
+           (△ γκu (1 / 2))
+           ∗
+           (EX γe ())
+           ∗
+           (▿ γr 0)
+           ∗
+           (Duty(tid2) [(κu, 0, (▿ γκu 0)%S)])
+           ∗
+           (◇{([(κu, 0)])%S}(1, 9)))%S, n⟧)
+      -∗
+  ⟦(syn_wpsim (S n) tid2 ⊤ (λ rs rt : Any.t, ( ⤉ syn_term_cond n tid2 Any.t rs rt)) false true
+    (trigger Yield;;; ` x : SCMem.val <- Ret (SCMem.val_nat 0);; Ret (Any.upcast x))
+    (` r : SCMem.val <- map_event (OMod.emb_callee omod (SCMem.mod gvs)) (SCMem.load_fun D);;
+     ` x : Any.t <- map_event (OMod.emb_callee omod (SCMem.mod gvs)) (Ret (Any.upcast r));;
+     ` x0 : SCMem.val <- (tau;; unwrap (Any.downcast x));;
+     ` x1 : () + () <-
+     OMod.close_itree omod (SCMem.mod gvs)
+       (` b : bool <- OMod.call "compare" (x0, 1 : SCMem.val);; ` r0 : () + () <- (if b then Ret (inr ()) else Ret (inl ()));; Ret r0);;
+     OMod.close_itree omod (SCMem.mod gvs)
+       match x1 with
+       | inl l =>
+           tau;; ITree.iter
+                   (λ _ : (),
+                      ` d : SCMem.val <- OMod.call "load" D;;
+                      ` b : bool <- OMod.call "compare" (d, 1 : SCMem.val);;
+                      ` r0 : () + () <- (if b then Ret (inr ()) else Ret (inl ()));; Ret r0) l
+       | inr r0 => Ret r0
+       end;;;
+     ` x3 : SCMem.val <- OMod.close_itree omod (SCMem.mod gvs) ((trigger Yield;;; Spinlock.unlock X);;; trigger Yield;;; Ret (0 : SCMem.val));;
+            OMod.close_itree omod (SCMem.mod gvs) (Ret (Any.upcast x3))))%S, 1+n⟧.
+  Proof.
+    iEval (red_tl_all; rewrite red_syn_tgt_interp_as; rewrite red_syn_wpsim; simpl).
+    iIntros "#INV_CL #MEM #ISL (TID & #PRu & #LINKu & #Dl & #Dw & Lu & EX & #Dr & DUTY & PCS)".
+    iInv "INV_CL" as "CL" "INV_CL_CLOSE".
+    iPoseProof (data_case3_after with "Dl Dw Dr Lu CL") as "(LXw & PTD & Lu1 & Lu2)".
+    iApply (SCMem_load_fun_spec with "[PTD] [-]").
+    3:{ iSplitR. auto. iFrame. }
+    lia.
+    { pose md_N_ClientSpinlock2_state_tgt. set_solver. }
+    iIntros (rv) "[%RV PTD]". subst rv. rred2r. iApply wpsim_tauR. rred2r.
+    iMod ("INV_CL_CLOSE" with "[LXw Lu2 PTD]") as "_".
+    { iEval (unfold clientSpinlock2_inv; simpl; red_tl_all; simpl). do 2 iRight. iLeft. iFrame.
+      iExists _. iEval (red_tl). iExists _. iEval (red_tl). iExists _. iEval (red_tl_all; simpl).
+      iFrame. do 4 (iSplitR; [eauto | ]). iRight. auto.
+    }
+    iApply (wpsim_yieldR2 with "[DUTY PCS]").
+    3:{ iFrame. iFrame. }
+    1,2: lia.
+    iIntros "DUTY _ PCS". rred2r. 
+    iApply (SCMem_compare_fun_spec). auto. set_solver. simpl.
+    iApply (tgt_interp_as_equiv with "MEM").
+    { iIntros (a). iStartProof. simpl; red_tl_all; simpl. iSplit.
+      { iIntros "MB"; iSplit; iFrame. iPureIntro; auto. }
+      { iIntros "[MB _]"; iFrame. }
+    }
+    iIntros (rv) "[%EQ1 _]". specialize (EQ1 eq_refl). subst rv.
+    rred2r. iApply wpsim_tauR. rred2r.
+    iApply (wpsim_yieldR2 with "[DUTY PCS]").
+    3:{ iFrame. }
+    1,2: lia.
+    iIntros "DUTY _ PCS". rred2r. iApply wpsim_tauR. rred2r.
+
+    (* Unlock. *)
+    iPoseProof ((Spinlock_unlock_spec tid2 n ⊤) $! X γX γe κs ℓL) as "SPEC".
+    set (P0 := ((△ γκu (1/2)))%S : sProp n).
+    set (R0 := ((△ γκu (1/2)) ∗ Duty(tid2) [(κu, 0, (▿ γκu 0)%S)])%S : sProp n).
+    set (Q0 := ((▿ γκu 0) ∗ Duty(tid2) [])%S : sProp n).
+    iSpecialize ("SPEC" $! _ P0 R0 Q0).
+    iEval (simpl) in "PCS". iMod (pcs_decr _ _ 1 0 with "PCS") as "[PCS _]".
+    lia.
+    iApply ("SPEC" with "[EX Lu1 DUTY PCS] [-]").
+    { subst P0 R0 Q0. iEval (red_tl_all; simpl). do 2 (iSplitR; [auto | ]). iFrame. iFrame.
+      iSplitR.
+      { iIntros "(LX & Lu & DUTY)". iInv "INV_CL" as "CL" "INV_CL_CLOSE".
+        iPoseProof (data_case3_after with "Dl Dw Dr Lu CL") as "(LXw & PTD & Lu1 & Lu2)".
+        iMod (AuthExcls.b_w_update _ _ _ 0 with "LX LXw") as "[LX LXw]".
+        iMod (OneShots.pending_shot _ 0 with "[Lu1 Lu2]") as "#Du".
+        { iEval (replace 1%Qp with (1/2 + 1/2)%Qp by apply Qp.div_2). iApply (OneShots.pending_merge with "Lu1 Lu2"). }
+        iMod ("INV_CL_CLOSE" with "[LXw PTD]") as "_".
+        { iEval (unfold clientSpinlock2_inv; simpl; red_tl_all; simpl). do 3 iRight. iFrame.
+          iExists γκw. iEval (red_tl). iExists γκu. iEval (red_tl_all). auto.
+        }
+        iMod (duty_fulfill with "[DUTY]") as "DUTY".
+        { iFrame. iEval (simpl; red_tl_all). auto. }
+        iModIntro. iFrame. auto.
+      }
+      iSplitR.
+      { iModIntro. iIntros "(Lu & DUTY)". iModIntro. iFrame. }
+      { iModIntro. iIntros "(Lu & DUTY)". iModIntro. iFrame. }
+    }
+    subst Q0. iEval (red_tl_all; simpl). iIntros (_) "[Du DUTY]". rred2r.
+    iApply (wpsim_sync with "[DUTY]").
+    2:{ iFrame. }
+    lia.
+    iIntros "DUTY _". rred2r. iApply wpsim_tauR. rred2r. lred2r.
+    iApply wpsim_ret.
+    2:{ iModIntro. iFrame. iPureIntro. auto. }
+    reflexivity.
+  Qed.
+
+  Lemma loop_case3
         (tid2 n ℓL ℓl : nat)
         (LAYER_L : ℓL = 3)
         (LAYER_l : ℓl = 2)
@@ -506,15 +670,113 @@ Section SIM.
                                     (ITree.iter
                                        (λ _ : (),
                                            ` d : SCMem.val <- OMod.call "load" D;;
-                                                 ` b : bool <- OMod.call "compare" (d, 1);; ` r : () + () <- (if b then Ret (inr ()) else Ret (inl ()));; Ret r) ());;;
-                                    x <- OMod.close_itree omod (SCMem.mod gvs) ((trigger Yield;;; Spinlock.unlock X);;; Ret (0 : SCMem.val));;
-                   OMod.close_itree omod (SCMem.mod gvs) (Ret (Any.upcast x))))%S, 1+n⟧
+                                                 ` b : bool <- OMod.call "compare" (d, 1 : SCMem.val);; ` r : () + () <- (if b then Ret (inr ()) else Ret (inl ()));; Ret r) ());;;
+                                    ` x : SCMem.val <- OMod.close_itree omod (SCMem.mod gvs) ((trigger Yield;;; Spinlock.unlock X);;; trigger Yield;;; Ret (0 : SCMem.val));;
+                                          OMod.close_itree omod (SCMem.mod gvs) (Ret (Any.upcast x)))
+       )%S, 1+n⟧
   .
   Proof.
     iEval (red_tl_all; rewrite red_syn_tgt_interp_as; rewrite red_syn_wpsim; simpl).
     iIntros "#INV_CL #MEM #ISL (TID & #PRu & #LINKu & #Dl & #Dw & Lu & EX & #Dr & DUTY & PC)".
+    iEval (rewrite unfold_iter_eq). rred2r.
+    iApply (wpsim_yieldR2 with "[DUTY PC]").
+    3:{ iFrame. iFrame. }
+    1,2: lia.
+    iIntros "DUTY _ PCS". rred2r.
+    iPoseProof (loop_case3_in with "INV_CL [MEM] ISL [-]") as "SIM".
+    5:{ iEval (rewrite red_syn_wpsim) in "SIM". iFrame. }
+    1,2: auto.
+    { iEval (rewrite red_syn_tgt_interp_as). auto. }
+    iEval (red_tl_all; simpl). iFrame. eauto.
+  Qed.
+
+  Lemma data_case2 n γX γκl tid2 κs ℓL :
+    ((○ γX 1) ∗ (D ↦ 0) ∗
+              (∃ x : nat,
+                  ⟦ ∃ γκw : τ{nat}, -[x](0)-◇ (∃ γκu : τ{nat}, ▿ γκw γκu) ∗ (△ γκw (1 / 2)) ∗ (▿ γκl γκw) ∗ Duty(tid2) [] ∗ ◇[κs](ℓL, 1) ∗
+                                            (∃ ℓw : τ{nat}, ◆[x, ℓw] ∗ ⌜ℓw ≤ ℓL⌝), n ⟧))
+      ⊢
+      ((○ γX 1) ∗ (D ↦ 0) ∗
+                (∃ κw γκw,
+                    ⟦ (-[κw](0)-◇ (∃ γκu : τ{nat}, ▿ γκw γκu) ∗ (△ γκw (1 / 2)) ∗ (▿ γκl γκw) ∗ Duty(tid2) [] ∗ ◇[κs](ℓL, 1) ∗
+                                  (∃ ℓw : τ{nat}, ◆[κw, ℓw] ∗ ⌜ℓw ≤ ℓL⌝))%S, n ⟧)).
+  Proof.
+    iIntros "CL2". iDestruct "CL2" as "(LXw & PTD & %κw & CL2)". iEval (red_tl) in "CL2". iDestruct "CL2" as "[%γκw CL2]".
+    iEval (red_tl_all; simpl) in "CL2". iDestruct "CL2" as "(#PROM_w & LIVE_w & #DEAD_l & DUTY2 & PC_spin & LO_w)".
+    iFrame. iExists κw, γκw. iEval (red_tl_all; simpl). iFrame. eauto.
+  Qed.
+
+  Lemma loop_case2
+        (tid2 n ℓL ℓl : nat)
+        (LAYER_L : ℓL = 3)
+        (LAYER_l : ℓl = 2)
+        (γX γe κs κl γκl γr κw ℓw : nat)
+        (γκw : nat)
+        (LAYw : ℓw ≤ ℓL)
+    :
+    ⊢
+      (inv n N_ClientSpinlock2 (clientSpinlock2_inv n tid2 ℓL ℓl γX γe κs κl γκl γr))
+      -∗
+      (⟦(syn_tgt_interp_as n sndl (λ m : SCMem.t, s_memory_black m))%S, 1+n⟧)
+      -∗
+      (⟦ isSpinlock n X γX γe κs ℓL, n ⟧)
+      -∗
+      (⟦(-[κw](0)-◇ (∃ γκu : τ{nat}, ▿ γκw γκu))%S, n⟧)
+      -∗
+      (▿ γκl γκw)
+      -∗
+      (◆[κw, ℓw])
+      -∗
+      (own_thread tid2)
+      -∗
+      (△ γr 1)
+      -∗
+      ((○ γX 1) ∗ (D ↦ 0) ∗
+                (∃ x : nat,
+                    ⟦ ∃ γκw0 : τ{nat}, -[x](0)-◇ (∃ γκu : τ{nat}, ▿ γκw0 γκu) ∗ (△ γκw0 (1 / 2)) ∗ (▿ γκl γκw0) ∗ Duty(tid2) [] ∗ ◇[κs](ℓL, 1) ∗
+                                               (∃ ℓw : τ{nat}, ◆[x, ℓw] ∗ ⌜ℓw ≤ ℓL⌝), n ⟧))
+      -∗
+      (prop n (clientSpinlock2_inv n tid2 ℓL ℓl γX γe κs κl γκl γr) =| S n |={ ⊤ ∖ ↑N_ClientSpinlock2, ⊤ }=∗ emp)
+      -∗
+      ⟦(syn_wpsim (S n) tid2 (⊤ ∖ ↑N_ClientSpinlock2) (λ rs rt : Any.t, (⤉ syn_term_cond n tid2 Any.t rs rt)) false true
+                  (trigger Yield;;; ` x : SCMem.val <- Ret (0 : SCMem.val);; Ret (Any.upcast x))
+                  (OMod.close_itree omod (SCMem.mod gvs)
+                                    (ITree.iter
+                                       (λ _ : (),
+                                           ` d : SCMem.val <- OMod.call "load" D;;
+                                                 ` b : bool <- OMod.call "compare" (d, 1);; ` r : () + () <- (if b then Ret (inr ()) else Ret (inl ()));; Ret r) ());;;
+                                    ` x : SCMem.val <- OMod.close_itree omod (SCMem.mod gvs) ((trigger Yield;;; Spinlock.unlock X);;; trigger Yield;;; Ret (0 : SCMem.val));;
+                                          OMod.close_itree omod (SCMem.mod gvs) (Ret (Any.upcast x))))%S, 1+n⟧
+  .
+  Proof.
+    iEval (red_tl_all; rewrite red_syn_tgt_interp_as; rewrite red_syn_wpsim; simpl).
+    iIntros "#INV_CL #MEM #ISL #PRw #Dl #LOw TID Lr CL2 INV_CL_CLOSE".
 
     TODO
+
+
+
+
+    iMod ("INV_CL_CLOSE" with "[LXw PTD Lw PCspin DUTY]") as "_".
+    { iEval (unfold clientSpinlock2_inv; simpl; red_tl_all; simpl). do 1 iRight. iLeft. iFrame.
+      iExists _. iEval (red_tl). iExists _. iEval (red_tl_all; simpl). iFrame. do 2 (iSplit; [auto|]).
+      iExists _. iEval (red_tl; simpl). eauto.
+    }
+
+
+    iPoseProof (data_case2 with "CL2") as "(LXw & PTD & % & % & CL2)". iEval (red_tl_all; simpl) in "CL2".
+    iDestruct "CL2" as "(_ & Lw & #Dl2 & DUTY & PCspin & _)".
+    iPoseProof (OneShots.shot_agree with "Dl Dl2") as "%EQ". subst γκw0. iClear "Dl2".
+    
+    
+tpromise_ind2:
+  ∀ {ident_tgt : Type} {Vars : nat → Type} {Σ : GRA.t} {Invs : IInvSet Vars} {IDENTTGT : GRA.inG (identTgtRA ident_tgt) Σ} 
+    {OBLGRA : GRA.inG ObligationRA.t Σ} {ONESHOTRA : GRA.inG ArrowShotRA Σ} {ARROWRA : GRA.inG (ArrowRA ident_tgt) Σ} 
+    (v k l m : nat) (f : Vars v) (R : iProp),
+    ◆[k, l] ∗ -[k](m)-◇ f -∗ □ ((€ =( ObligationRA.arrows_sat v )=∗ R) ==∗ R) ∗ □ (□ prop v f ==∗ R) ==∗ R
+    
+    
+    
 
 
   Lemma ClientSpinlock2_thread2_sim
@@ -559,41 +821,49 @@ Section SIM.
         3:{ iFrame. iApply pcs_cons_fold. iFrame. }
         1,2: lia.
         iIntros "DUTY _ PCS". rred2r. iApply wpsim_tauR. rred2r.
+        iMod (pcs_decr _ _ 10 0 with "PCS") as "[PCS _]".
+        lia.
+        iPoseProof (loop_case3 with "INV_CL [MEM] ISL [-]") as "SIM".
+        5:{ iEval (rewrite red_syn_wpsim) in "SIM". iFrame. }
+        1,2: auto.
+        { iEval (rewrite red_syn_tgt_interp_as). auto. }
+        iEval (red_tl_all; simpl). iFrame.
+    }
+    2:{ iPoseProof (data_case2 with "CL2") as "(LXw & PTD & % & % & CL2)". iEval (red_tl_all; simpl) in "CL2".
+        iDestruct "CL2" as "(#PRw & Lw & #Dl & DUTY & PCspin & (% & LO))".
+        iEval (red_tl_all; simpl) in "LO". iDestruct "LO" as "[#LOw %LAYw]".
+        iApply (wpsim_yieldR_gen with "[DUTY]").
+        2: iFrame.
+        lia.
+        iIntros "DUTY _". iMod ("INV_CL_CLOSE" with "[LXw PTD Lw PCspin DUTY]") as "_".
+        { iEval (unfold clientSpinlock2_inv; simpl; red_tl_all; simpl). do 1 iRight. iLeft. iFrame.
+          iExists _. iEval (red_tl). iExists _. iEval (red_tl_all; simpl). iFrame. do 2 (iSplit; [auto|]).
+          iExists _. iEval (red_tl; simpl). eauto.
+        }
+        iModIntro. rred2r. iApply wpsim_tauR. rred2r.
+        iInv "INV_CL" as "CL" "INV_CL_CLOSE".
+        iEval (unfold clientSpinlock2_inv; simpl; red_tl_all; simpl) in "CL".
+        iDestruct "CL" as "[CL1 | [CL2 | [CL3 | CL4]]]".
+        4:{ iPoseProof (not_case4 with "CL4 LIVE_r") as "%F". inv F. }
+        3:{ iMod (data_case3 with "CL3 LIVE_r") as "((%γκw0 & %κu & %γκu & A) & #Dr & CL3)".
+            iMod ("INV_CL_CLOSE" with "[CL3]") as "_".
+            { iEval (unfold clientSpinlock2_inv; simpl; red_tl_all; simpl). do 2 iRight. iLeft. iFrame. }
+            iEval (red_tl_all; simpl) in "A". iDestruct "A" as "(PRu & LINKu & #Dl2 & #Dw & DUTY & PC & Lu & EX)".
+            iPoseProof (OneShots.shot_agree with "Dl Dl2") as "%EQ". subst γκw0.
+            iMod (pc_drop _ 1 _ _ 10 with "PC") as "PC".
+            Unshelve. 1,3: lia.
+            iPoseProof (pcs_cons_fold _ 0 [] 1 10 with "[PC]") as "PCS".
+            { iFrame. }
+            iPoseProof (loop_case3 with "INV_CL [MEM] ISL [-]") as "SIM".
+            5:{ iEval (rewrite red_syn_wpsim) in "SIM". iFrame. }
+            1,2: auto.
+            { iEval (rewrite red_syn_tgt_interp_as). auto. }
+            iEval (red_tl_all; simpl). iFrame. eauto.
+        }
+        2:{ 
 
 
 
-
-
-
-  Definition clientSpinlock2_inv n (tid2 : thread_id) (ℓL ℓl : nat) (γX γe κs : nat) (κl γκl : nat) (γr : nat) : sProp n :=
-    (
-      ((○ γX 0) ∗ (D ↦ 0)
-                ∗ (-[κl](0)-◇ (∃ (γκw : τ{nat}), ▿ γκl γκw)) ∗ (△ γκl (1/2))
-                ∗ (Duty(tid2) [])
-                ∗ ◇[κs](ℓL, 1)
-                ∗ (∃ (ℓl : τ{nat}), ◆[κl, ℓl])
-      )
-      ∨
-        ((○ γX 1) ∗ (D ↦ 0)
-                  ∗ (∃ (κw γκw : τ{nat}),
-                        (-[κw](0)-◇ (∃ (γκu : τ{nat}), (▿ γκw γκu)))
-                          ∗ (△ γκw (1/2)) ∗ (▿ γκl γκw)
-                          ∗ (Duty(tid2) [])
-                          ∗ ◇[κs](ℓL, 1)
-                          ∗ (∃ (ℓw : τ{nat}), ◆[κw, ℓw] ∗ ⌜ℓw <= ℓL⌝))
-        )
-      ∨
-        ((○ γX 1) ∗ (D ↦ 1)
-                  ∗ (∃ (γκw κu γκu : τ{nat}),
-                        (-[κu](0)-◇ (▿ γκu 0))
-                          ∗ (△ γκu (1/2)) ∗ (κu -(0)-◇ κs) ∗ (▿ γκl γκw) ∗ (▿ γκw γκu)
-                          ∗ ((Duty(tid2) [(κu, 0, (▿ γκu 0))] ∗ ◇[κu](ℓl, 1) ∗ (△ γκu (1/2)) ∗ (EX γe tt)) ∨ (▿ γr 0)))
-        )
-      ∨
-        ((○ γX 0) ∗ (D ↦ 1)
-                  ∗ (∃ (γκw γκu : τ{nat}),
-                        (▿ γκl γκw) ∗ (▿ γκw γκu) ∗ (▿ γr 0) ∗ (▿ γκu 0)))
-    )%S.
 
 End SIM.
 
